AwsCryptographicMaterialProviders/dafny/AwsCryptographyKeyStoreAdmin/test/Mutations/TestInitMutActiveAndBeaconAreInSameState.dfy
@@ -35,6 +35,9 @@ module {:options "/functionSyntax:4" } TestInitMutActiveAndBeaconAreInSameState 
   const logicalName: string := Fixtures.logicalKeyStoreName
   const testLogPrefix := "\nTestMutationsActiveAndBeaconAreInSameState :: TestSadCase :: "
 
+  function {:opaque} TestLie(): set<object>
+  {{}}
+
   method {:test} {:vcs_split_on_every_assert} TestSadCase()
   {
     print " running";
@@ -42,16 +45,17 @@ module {:options "/functionSyntax:4" } TestInitMutActiveAndBeaconAreInSameState 
     // expect false; // disable test till other investigation is done
     var ddbClient :- expect DDB.DynamoDBClient();
     var kmsClient :- expect KMS.KMSClient();
-
+    var storage :- expect AdminFixtures.DefaultStorage(ddbClient?:=Some(ddbClient));
     var underTest :- expect AdminFixtures.DefaultAdmin(ddbClient?:=Some(ddbClient));
     var strategy :- expect AdminFixtures.DefaultKeyManagerStrategy(kmsClient?:=Some(kmsClient));
     // Recommend commenting this out while developing this method,
     // and just ignore the modifies exeptions,
     // and then re-enabling it once everything is safe
-    // assume {:axiom} underTest.Modifies == {};
+    assume {:axiom} underTest.Modifies == {} && storage.Modifies == {};
+    assume {:axiom} underTest.Modifies < TestLie(); // This does not work... but I have it here
 
-    // var uuid :- expect UUID.GenerateUUID();
-    var testId := sadCaseId; // + "-" + uuid;
+    var uuid :- expect UUID.GenerateUUID();
+    var testId := sadCaseId + "-" + uuid;
 
     var kodaBytes :- expect UTF8.Encode("Koda");
     var isADogBytes :- expect UTF8.Encode("is a dog.");
@@ -79,12 +83,25 @@ module {:options "/functionSyntax:4" } TestInitMutActiveAndBeaconAreInSameState 
         expect true;
       case _ => expect false, "Initialize Mutation should fail with Unexpected State Exception if Active & Beacon are different!";
     }
-    print testLogPrefix + " Initialize Mutation met expectations\n";
+    print testLogPrefix + " Initialize Mutation met expectations. Cleaning up\n";
+
+    var _ := CleanupItems.DeleteTypeWithFailure(testId, Structure.BEACON_KEY_TYPE_VALUE, ddbClient);
+    var _ := CleanupItems.DeleteTypeWithFailure(testId, Structure.BRANCH_KEY_ACTIVE_TYPE, ddbClient);
+
+    var versionQuery := KeyStoreTypes.QueryForVersionsInput(
+      Identifier := testId, pageSize := 24
+    );
+    var queryOut :- expect storage.QueryForVersions(versionQuery);
+    var items := queryOut.items;
+    var itemIndex := 0;
+    while itemIndex < |items|
+    {
+      expect "type" in items[itemIndex].EncryptionContext, "Decrypt Only item is missing 'type' from EC!!";
+      var _ := CleanupItems.DeleteTypeWithFailure(testId, items[itemIndex].EncryptionContext["type"], ddbClient);
+      itemIndex := itemIndex + 1;
+    }
+
     print "TestInitMutActiveAndBeaconAreInSameState.TestSadCase: ";
+
   }
 }
-// testId: test-mutate-encryption-add-value-da72ac87-5d28-4b84-8a56-96b4ea6e4326
-
-// TestEncryptionContextAddValue :: TestHappyCase ::  Violated the active and latest. testId: test-mutate-encryption-add-value-da72ac87-5d28-4b84-8a56-96b4ea6e4326
-
-        // dafny/AwsCryptographyKeyStoreAdmin/test/Mutations/TestEncryptionContextAddValue.dfy(89,28): Wrappers.Result.Failure(AwsCryptographyKeyStoreAdminTypes.Error.UnexpectedStateException(Beacon Item is not in the Original State! For Initialize Mutation to succeed, the ACTIVE & Beacon Key MUST be in the original state.))
